src/simple-proof/Safety.v
@@ -27,13 +27,115 @@ Inductive normal_form: trm -> Prop :=
 
 Hint Constructors normal_form.
 
-(*
-Let G |- t: T and G ~ s. Then either
+Lemma preservation: forall G s t s' t' T,
+    G ~~ s ->
+    inert G ->
+    t / s => t' / s' ->
+    G |- t : T ->
+    exists G', inert G' /\
+          G & G' ~~ s' /\
+          G & G' |- t' : T.
+Proof.
+  introv Hwf Hin Hred Ht.
+  gen t'.
+  dependent induction Ht; intros; try solve [inversions Hred].
+  - pose proof (canonical_forms_1 Hwf Hin Ht1) as [L [T' [t [Bis [Hsub Hty]]]]].
+    inversions Hred. 
+    apply (binds_func H4) in Bis. inversions Bis.
+    exists (@empty typ). rewrite concat_empty_r. repeat split; auto.
+    pick_fresh y. assert (y \notin L) as FrL by auto. specialize (Hty y FrL).
+    rewrite subst_intro_typ with (x:=y); auto. 
+    rewrite subst_intro_trm with (x:=y); auto.
+    eapply subst_ty_trm; eauto. rewrite~ subst_fresh_typ. 
+  - pose proof (canonical_forms_2 Hin Hwf Ht) as [S [ds [t [Bis [Has Ty]]]]].
+    inversions Hred.
+    apply (binds_func H1) in Bis. inversions Bis.
+    exists (@empty typ). rewrite concat_empty_r. repeat split; auto.
+    rewrite <- (defs_has_inv Has H5). assumption.
+  - destruct t.
+    + inversions Hred; try solve [inversion H6].
+      pick_fresh y. 
+      exists (@empty typ). rewrite concat_empty_r. repeat split; auto.
+      rewrite subst_intro_trm with (x:=y); auto.
+      rewrite <- subst_fresh_typ with (x:=y) (y:=x); auto.
+      eapply subst_ty_trm; eauto. rewrite~ subst_fresh_typ.
+    + inversions Hred; try solve [inversion H6].
+      pose proof (wf_sto_notin_dom Hwf H6).
+      pose proof (val_typing Ht) as [V [Hv Hs]].
+      pick_fresh y. assert (y \notin L) by auto.
+      specialize (H y H2).
+      exists (x ~ V). repeat split. 
+      * rewrite <- concat_empty_l. constructor~.
+        apply (precise_inert_typ Hv).
+      * constructor~. 
+        apply (precise_to_general Hv).
+      * rewrite subst_intro_trm with (x:=y); auto.
+        rewrite <- subst_fresh_typ with (x:=y) (y:=x); auto.
+        eapply subst_ty_trm; eauto. 
+        { eapply weaken_rules; eauto. }
+        { apply~ fv_ctx_types_push. }
+        { rewrite~ subst_fresh_typ. 
+          pose proof (ty_var (binds_tail x V G)).
+          apply (ty_sub H3). apply (weaken_subtyp Hs); eauto. 
+        }
+    + inversions Hred. 
+      specialize (IHHt Hwf Hin t0' H6) as [G' [Hin' [Hwf' Ht']]].
+      exists G'. repeat split; auto.
+      apply_fresh ty_let as z; eauto. 
+      eapply weaken_rules; eauto.
+    + inversions Hred. 
+      specialize (IHHt Hwf Hin t0' H6) as [G' [Hin' [Hwf' Ht']]].
+      exists G'. repeat split; auto.
+      apply_fresh ty_let as z; eauto. 
+      eapply weaken_rules; eauto.
+    + inversions Hred. 
+      specialize (IHHt Hwf Hin t0' H6) as [G' [Hin' [Hwf' Ht']]].
+      exists G'. repeat split; auto.
+      apply_fresh ty_let as z; eauto. 
+      eapply weaken_rules; eauto.
+  - specialize (IHHt Hwf Hin t' Hred) as [G' [Hin' [Hwf' Ht']]].
+    exists G'. repeat split; auto.
+    apply weaken_subtyp with (G2:=G') in H.
+    + apply (ty_sub Ht' H).
+    + eauto.
+Qed.
 
-- t is a normal form, or
-- there exists a store s', term t' such that s | t -> s' | t', and for any such s', t' there exists an environment G'' such that, letting G' = G, G'' one has G' |- t': T and G' ~ s'.
-The proof is by a induction on typing derivations of G |- t: T.
-*)
+Lemma progress: forall G t s T,
+    G ~~ s ->
+    inert G ->
+    G |- t : T ->
+    (normal_form t \/ exists t' s', t / s => t' / s').
+Proof.
+  introv Hwf Hin Ht. dependent induction Ht; try solve [left; auto].
+  - pose proof (canonical_forms_1 Hwf Hin Ht1) as [L [T' [t [Bis [Hsub Hty]]]]].
+    right. exists (open_trm z t) s.
+    eapply red_app; eauto.
+  - pose proof (canonical_forms_2 Hin Hwf Ht) as [S [ds [t [Bis [Has Ty]]]]].
+    right. exists t s.
+    eapply red_sel; eauto.
+  - right. destruct t.
+    + pose proof (var_typing_implies_avar_f Ht) as [x A]. subst.
+      exists (open_trm x u) s.
+      apply red_let_var.
+    + pick_fresh x.
+      exists (open_trm x u) (s & x ~ v).
+      eapply red_let; auto.
+    + specialize (IHHt Hwf Hin) as [IH | [t' [s' Hred]]].
+      * inversion IH.
+      * exists (trm_let t' u) s'.
+        apply~ red_let_tgt.
+    + specialize (IHHt Hwf Hin) as [IH | [t' [s' Hred]]].
+      * inversion IH.
+      * exists (trm_let t' u) s'.
+        apply~ red_let_tgt.
+    + specialize (IHHt Hwf Hin) as [IH | [t' [s' Hred]]].
+      * inversion IH.
+      * exists (trm_let t' u) s'.
+        apply~ red_let_tgt.
+  - specialize (IHHt Hwf Hin) as [IH | [t' [s' Hred]]].
+    + left. assumption.
+    + right. exists t' s'. assumption.
+Qed.
 
 Lemma safety: forall G s t T,
     G ~~ s ->
@@ -56,8 +158,7 @@ Proof.
     eapply subst_ty_trm. eapply Hty.
     apply ok_push. eapply wf_sto_to_ok_G. eassumption. eauto. eauto.
     rewrite subst_fresh_typ.
-    apply ty_sub with (T:=S).
-    assumption. apply subtyp_refl.
+    assumption. 
     eauto. eauto. eauto. eauto.
   - (* Fld-E *) right.
     pose proof (canonical_forms_2 Hg Hwf H) as [S [ds [t [Bis [Has Ty]]]]].
